Nuova definizione, più debole di equivalenza tra stati per dimostrare correttezza compiler_v2

MasterThesis/Compiler/Compiler_v2.lean
@@ -1,21 +1,15 @@
 import MasterThesis.SCORE.Language
 import MasterThesis.LOOP.Language
 
-namespace SCORE
-
-open SCORE Com
-
-def l2s' (ev : Ident) (Lc: LOOP.Com) : SCORE.Com :=
-  match Lc with
-  | LOOP.Com.SKIP    => SKIP
-  | LOOP.Com.ZER x   => CON x
-  | LOOP.Com.ASN x y => FOR y (INC ev) ;;
-                        CON x ;;
-                        FOR ev (INC x) ;;
-                        FOR x (DEC ev)
-  | LOOP.Com.INC x   => INC x
-  | LOOP.Com.SEQ P Q => l2s' ev P ;;
+def l2s' (ev : Ident) (P : LOOP.Com) : SCORE.Com :=
+  match P with
+  | LOOP.Com.SKIP    => SCORE.Com.SKIP
+  | LOOP.Com.ZER x   => SCORE.Com.CON x
+  | LOOP.Com.ASN x y => SCORE.Com.FOR y (SCORE.Com.INC ev);;
+                        SCORE.Com.CON x;;
+                        SCORE.Com.FOR ev (SCORE.Com.INC x);;
+                        SCORE.Com.FOR x (SCORE.Com.DEC ev)
+  | LOOP.Com.INC x   => SCORE.Com.INC x
+  | LOOP.Com.SEQ P Q => l2s' ev P;;
                         l2s' ev Q
-  | LOOP.Com.FOR x P => FOR x (l2s' ev P)
-
-end SCORE
+  | LOOP.Com.FOR x P => SCORE.Com.FOR x (l2s' ev P)
